AnnotatedFix.v
@@ -7,7 +7,7 @@ Require Export SystemFR.NatCompareErase.
 
 Opaque reducible_values.
 
-Lemma annotated_reducible_fix:
+Lemma annotated_reducible_fix_strong_induction:
   forall tvars gamma ts T n y p,
     ~(n ∈ fv_context gamma) ->
     ~(y ∈ fv_context gamma) ->
@@ -28,53 +28,10 @@ Lemma annotated_reducible_fix:
     subset (fv ts) (support gamma) ->
     is_annotated_type T ->
     is_annotated_term ts ->
+    cbv_value (erase_term ts) ->
     [[ tvars;
-        (p, T_equiv (fvar y term_var) (lambda T_unit (tfix T ts))) ::
-        (y, T_arrow T_unit (open 0 T (fvar n term_var))) ::
-        (n, T_nat) ::
-        gamma ⊨
-          open 0 (open 1 ts (succ (fvar n term_var))) (fvar y term_var) :
-          open 0 T (succ (fvar n term_var))
-    ]] ->
-    [[ tvars; (y, T_top) :: gamma ⊨
-        open 0 (open 1 ts zero) (fvar y term_var) :
-        open 0 T zero ]]
-    ->
-    [[ tvars; gamma ⊨ tfix T ts : T_forall T_nat T ]].
-Proof.
-  unfold annotated_reducible; steps.
-  apply open_reducible_fix with n y p;
-    repeat step || erase_open || rewrite (open_none (erase_term ts)) in * by auto;
-    side_conditions.
-Qed.
-
-Lemma annotated_reducible_fix_strong_induct:
-  forall tvars gamma ts T n y p,
-    ~(n ∈ fv_context gamma) ->
-    ~(y ∈ fv_context gamma) ->
-    ~(p ∈ fv_context gamma) ->
-    ~(n ∈ fv T) ->
-    ~(n ∈ fv ts) ->
-    ~(y ∈ fv T) ->
-    ~(y ∈ fv ts) ->
-    ~(p ∈ fv T) ->
-    ~(p ∈ fv ts) ->
-    ~(n ∈ tvars) ->
-    ~(y ∈ tvars) ->
-    ~(p ∈ tvars) ->
-    NoDup (n :: y :: p :: nil) ->
-    wf (erase_term ts) 1 ->
-    wf T 1 ->
-    subset (fv T) (support gamma) ->
-    subset (fv ts) (support gamma) ->
-    is_annotated_type T ->
-    is_annotated_term ts ->
-    [[ tvars;
-        (p, T_equiv (fvar y term_var) (lambda T_unit (tfix T ts))) ::
-        (y,
-          (T_forall
-             (T_refine T_nat (annotated_tlt (lvar 0 term_var) (fvar n term_var)))
-             (T_arrow T_unit (shift 0 T 1)))) ::
+        (p, T_equiv (fvar y term_var) (tfix T ts)) ::
+        (y, T_forall (T_refine T_nat (annotated_tlt (lvar 0 term_var) (fvar n term_var))) T) ::
         (n, T_nat) ::
         gamma ⊨
         open 0 (open 1 ts (fvar n term_var)) (fvar y term_var) :
@@ -89,4 +46,3 @@ Proof.
            (rewrite erase_type_shift in *);
     side_conditions.
 Qed.
-
